seiostar/LogRelSourceTarget.CompatibilityLemmas.fst
@@ -885,7 +885,7 @@ let helper_compat_oprod_openfile_oval_steps (h:history) (lt:local_trace h) (fs_f
 let compat_oprod_openfile_oval #g (fs_fnm:fs_oval g qString) (fnm:exp)
   : Lemma
     (requires fs_fnm ⊏ fnm)
-    (ensures fs_oprod_openfile_oval fs_fnm ⊑ EOpen fnm)
+    (ensures fs_oprod_call_oval OOpen fs_fnm ⊑ EOpen fnm)
   =
   lem_fv_in_env_openfile g fnm;
   introduce forall b (s:gsub g b) (fsG:eval_env g) (h:history). fsG `(≍) h` s ==> (qFileDescr ^+ qUnit) ⫃ (h, io_call OOpen (fs_fnm fsG), gsubst s (EOpen fnm)) with begin
@@ -933,7 +933,7 @@ let helper_compat_oprod_read_oval_steps (h:history) (lt:local_trace h) (fs_fd:fs
 let compat_oprod_read_oval #g (fs_fd:fs_oval g qFileDescr) (fd:exp)
   : Lemma
     (requires fs_fd ⊏ fd)
-    (ensures fs_oprod_read_oval fs_fd ⊑ ERead fd)
+    (ensures fs_oprod_call_oval ORead fs_fd ⊑ ERead fd)
   =
   lem_fv_in_env_read g fd;
   introduce forall b (s:gsub g b) (fsG:eval_env g) (h:history). fsG `(≍) h` s ==> (qString ^+ qUnit) ⫃ (h, io_call ORead (fs_fd fsG), gsubst s (ERead fd)) with begin
@@ -990,7 +990,7 @@ let helper_compat_oprod_write_oval_steps (h:history) (lt:local_trace h) (fs_fd:f
 let compat_oprod_write_oval #g (fs_fd:fs_oval g qFileDescr) (fs_msg:fs_oval g qString) (fd msg:exp)
   : Lemma
     (requires fs_fd ⊏ fd /\ fs_msg ⊏ msg)
-    (ensures fs_oprod_write_oval fs_fd fs_msg ⊑ EWrite fd msg)
+    (ensures fs_oprod_call_oval OWrite (fs_oval_pair fs_fd fs_msg) ⊑ EWrite fd msg)
   =
   lem_fv_in_env_write g fd msg;
   introduce forall b (s:gsub g b) (fsG:eval_env g) (h:history). fsG `(≍) h` s ==> (qUnit ^+ qUnit) ⫃ (h, io_call OWrite (fs_fd fsG, fs_msg fsG), gsubst s (EWrite fd msg)) with begin
@@ -1039,7 +1039,7 @@ let helper_compat_oprod_close_oval_steps (h:history) (lt:local_trace h) (fs_fd:f
 let compat_oprod_close_oval #g (fs_fd:fs_oval g qFileDescr) (fd:exp)
   : Lemma
     (requires fs_fd ⊏ fd)
-    (ensures fs_oprod_close_oval fs_fd ⊑ EClose fd)
+    (ensures fs_oprod_call_oval OClose fs_fd ⊑ EClose fd)
   =
   lem_fv_in_env_close g fd;
   introduce forall b (s:gsub g b) (fsG:eval_env g) (h:history). fsG `(≍) h` s ==> (qUnit ^+ qUnit) ⫃ (h, io_call OClose (fs_fd fsG), gsubst s (EClose fd)) with begin
